\input{preamble}

\begin{document}
\maketitle

\begin{dimo}[$x^n < y$]

	\begin{equation}
	x^n < y \ \iff\ \exists\epsilon \in \R, 
	\epsilon > 0 \ :\ (x + \epsilon)^n < y
	\end{equation}
Sia $\epsilon \in ]0,1[$

	\begin{equation}
	(x + \epsilon)^n\ =\ ((x + \epsilon)^n - x^n) + x^n\ =\
	((\xout{x} + \epsilon)- \xout{x})((x+ \epsilon)^{n-1}\ +\	
	\dots\ +\ x^{n-1}) + x^n\
	\end{equation}
	
	\begin{equation}
	\big\Downarrow
	\end{equation}

	\begin{equation}
	\epsilon ( (x + \epsilon)^{n-1} + \dots + x^{n-1}) + x^n\ \leq\
	\epsilon \cdot n \cdot (x + 1)^{n-1} + x^n
	\end{equation}

	\begin{equation}
	\big\Downarrow
	\end{equation}
	
	\begin{equation}
	\epsilon n (x+1)^{n-1} + x^n < y \ \iff\ 
	\epsilon < \frac{y - x^n}{n(x+1)^{n-1}} : \overset{def.}{=} \epsilon > 0
	\end{equation}

	\begin{equation}
	0\ <\ \epsilon\ <\ \frac{y - x^n}{n(x+1)^{n-1}} 	
	\end{equation}
Questo Ã¨ valido per: $ \epsilon \in \R $ 

		
\end{dimo}

\end{document}
